store/client_proofs/connect.v
@@ -5,7 +5,7 @@ From iris.algebra Require Import agree auth csum gset gmap excl frac.
 From iris.algebra Require Import max_prefix_list.
 From iris.heap_lang Require Import notation proofmode.
 From cryptis Require Import lib version term cryptis primitives tactics.
-From cryptis Require Import role session pk_auth pk_dh.
+From cryptis Require Import role dh_auth.
 From cryptis.store Require Import impl shared db.
 From cryptis.store.client_proofs Require Import common.
 
@@ -19,8 +19,6 @@ Context `{!cryptisGS Σ, !heapGS Σ, !sessionGS Σ, !storeGS Σ}.
 Notation iProp := (iProp Σ).
 
 Context `{!storeG Σ}.
-
-Local Instance STORE : PK := PK_DH (λ _ _ _ _, True)%I.
 
 Implicit Types (cs : cst).
 Implicit Types kI kR kS t : term.
@@ -36,60 +34,45 @@ Lemma wp_client_connect E c kI kR dq ph T :
   channel c -∗
   cryptis_ctx -∗
   store_ctx N -∗
-  public (TKey Enc kI) -∗
-  public (TKey Enc kR) -∗
+  public (TKey Dec kI) -∗
+  public (TKey Dec kR) -∗
   {{{ ●H{dq|ph} T }}}
-    Client.connect N c (TKey Dec kI) (TKey Enc kI) (TKey Enc kR) @ E
+    Client.connect N c (TKey Enc kI) (TKey Dec kI) (TKey Dec kR) @ E
   {{{ cs, RET (repr cs);
       ●H{dq|ph} T ∗
-      ⌜cst_ok cs = in_honest kI kR T⌝ ∗
-      client N cs }}}.
+      ⌜si_init cs = kI ∧ si_resp cs = kR ∧ si_time cs = ph ∧ si_hon cs = T⌝ ∗
+      client cs }}}.
 Proof.
 iIntros "% % #chan_c #ctx (#? & _ & _ & _ & _ & _ & _ & #ctx') #p_ekI #p_ekR".
 iIntros "!> %Φ hon post". rewrite /Client.connect. wp_pures.
 iCombine "hon post" as "post". iRevert "post".
 iApply wp_do_until. iIntros "!> [hon post]". wp_pures.
-wp_bind (pk_dh_init _ _ _ _ _).
-iApply (wp_pk_dh_init with "[] [] [] [] [] [hon]"); eauto.
-  by iFrame.
-iIntros "!> %okS [hon HokS]".
+wp_bind (initiator _ _ _ _ _).
+iMod (DB.alloc (bool_decide (TKey Enc kI ∈ T ∧ TKey Enc kR ∈ T)))
+  as "(%γ & auth & #frag)". wp_pures.
+iApply (wp_initiator γ with "[//] [//] [//] [] [] [hon]"); try solve_ndisj; eauto.
+iIntros "!> %okS (hon & HokS)".
 case: okS => [kS|]; wp_pures; last by iLeft; iFrame; eauto.
-wp_alloc timestamp as "ts". wp_pures. wp_tag.
-wp_bind (mkskey _). iApply wp_mkskey.
-iMod DB.alloc as "(%γ & auth & #frag)". wp_pures.
-iDestruct "HokS" as "(#s_kS & _ & #sessW & status)".
-set (ok := in_honest kI kR T).
-set (kS' := Spec.tag _ kS).
-iAssert (handshake_done N kS' ok) as "#done".
-  iExists kI, kR, kS, ph, T.
-  by do 2!iSplit => //.
-iAssert (|==> if ok then wf_key N kS' γ else True)%I
-  with "[status]" as ">#key".
-{ case e_ok: ok => //.
-  iDestruct "status" as "(#p_kS & token & #session)".
-  iMod (term_meta_set _ _ γ N with "token") as "#meta"; eauto.
-  iModIntro. iSplit.
-  - iIntros "!> %kt #p_kS'".
-    iPoseProof (public_sym_keyE with "[//] p_kS'") as ">contra".
-    by iDestruct ("p_kS" with "contra") as ">[]".
-  - iIntros "!> %kS'' %e".
-    case/Spec.tag_inj: e => _ <- {kS''}.
-    iExists kI, kR, ph, T. by eauto. }
+iDestruct "HokS" as "(#s_kS & #sessI & #key)".
+wp_alloc timestamp as "ts". wp_pures.
 wp_tsenc. wp_bind (send _ _).
 iApply (wp_send with "[#] [#]") => //.
   iModIntro. iApply public_TEncIS => //.
-  - by rewrite minted_TKey minted_tag.
-  - iModIntro. iExists ok, γ. by eauto.
+  - by rewrite minted_TKey.
+  - iModIntro. iExists _, γ. do !iSplit => //. by [].
   - by rewrite minted_TInt.
   - iIntros "!> _". by rewrite public_TInt.
 wp_pures. iRight. iExists _. iSplitR; eauto.
-iApply ("post" $! {| cst_ts := timestamp;
-                     cst_key := Spec.tag (nroot.@"keys".@"sym") kS;
-                     cst_name := γ;
-                     cst_ok := ok |}).
+set si := SessInfo _ _ _ _ _.
+iApply ("post" $! {| cst_si := si;
+                     cst_ts := timestamp;
+                     cst_name := γ |}).
 rewrite /client /=. iFrame. iModIntro. iSplit => //.
 iExists 0. iFrame. iSplit => //. iSplit => //.
-by rewrite minted_tag.
+rewrite /session_ok /=. iFrame. iSplit => //.
+set b1 := bool_decide _. set b2 := bool_decide _.
+suff -> : b1 = b2 by [].
+by apply: bool_decide_ext.
 Qed.
 
 End Verif.
