store/client_proofs/create.v
@@ -5,7 +5,7 @@ From iris.algebra Require Import agree auth csum gset gmap excl frac.
 From iris.algebra Require Import max_prefix_list.
 From iris.heap_lang Require Import notation proofmode.
 From cryptis Require Import lib version term cryptis primitives tactics.
-From cryptis Require Import role session pk_auth pk_dh.
+From cryptis Require Import role dh_auth.
 From cryptis.store Require Import impl shared db.
 From cryptis.store.client_proofs Require Import common.
 
@@ -19,8 +19,6 @@ Context `{!cryptisGS Σ, !heapGS Σ, !sessionGS Σ, !storeGS Σ}.
 Notation iProp := (iProp Σ).
 
 Context `{!storeG Σ}.
-
-Local Instance STORE : PK := PK_DH (λ _ _ _ _, True)%I.
 
 Implicit Types (cs : cst).
 Implicit Types kI kR kS t : term.
@@ -36,10 +34,10 @@ Lemma wp_client_create E c cs t1 t2 :
   store_ctx N -∗
   public t1 -∗
   public t2 -∗
-  {{{ client N cs }}}
+  {{{ client cs }}}
     Client.create N c (repr cs) t1 t2 @ E
   {{{ (b : bool), RET #b;
-      client N cs ∗
+      client cs ∗
       if b then rem_mapsto cs t1 t2 else True }}}.
 Proof.
 iIntros "% #chan_c (_ & _ & _ & _ & _ & #? & #? & _)
@@ -59,7 +57,7 @@ iMod (DB.create_client t1 t2 with "client")
 wp_bind (send _ _). iApply wp_send => //.
 { iApply public_TEncIS => //.
   - by rewrite minted_TKey.
-  - iModIntro. iExists (cst_name cs), n, t1, t2, (cst_ok cs).
+  - iModIntro. iExists n, t1, t2, cs, (cst_name cs).
     by eauto 8.
   - rewrite minted_of_list /= minted_TInt.
     rewrite -[minted t1]public_minted -[minted t2]public_minted.
@@ -84,20 +82,19 @@ iApply (wp_client_incr_timestamp with "ts").
 iIntros "!> ts".
 iDestruct (public_TEncE with "p_m [//]") as "{p_m} [[pub p_m]|p_m]".
 - wp_pures. wp_bind (tint _). iApply wp_tint. wp_pures.
-  case is_ok: cst_ok.
-  { iDestruct "key" as "[#contra _]".
-    iDestruct ("contra" with "pub") as ">[]". }
+  iPoseProof ("key" with "pub") as ">%not_ok".
   wp_bind (eq_term _ _). iApply wp_eq_term. wp_pures.
   iModIntro. iRight. iExists _. iSplit => //.
   iApply "post".
   iPoseProof (DB.create_client_fake t1 t2 with "client") as "#fake".
   iSplitL => //; last first.
-  { rewrite /rem_mapsto is_ok. by case: bool_decide. }
-  iExists (S n). rewrite is_ok. iFrame. by eauto.
+  { rewrite /rem_mapsto (bool_decide_eq_false_2 _ not_ok).
+    by case: bool_decide. }
+  iExists (S n). iFrame. by eauto.
 - iDestruct "p_m" as "(#p_m & _)".
   wp_pures. wp_bind (tint _). iApply wp_tint. wp_pures.
-  iDestruct "p_m" as "(%n' & %t1' & %t2' & %b' & %ok & %e &
-                       done' & free)".
+  iDestruct "p_m" as "(%n' & %t1' & %t2' & %b' & %si & %γ' & %e & %e_key &
+                       sessR & free)".
   case/Spec.of_list_inj: e => en <- _ ->.
   have {en} <- : n = n' by lia.
   wp_bind (eq_term _ _).
@@ -109,11 +106,11 @@ iDestruct (public_TEncE with "p_m [//]") as "{p_m} [[pub p_m]|p_m]".
   iSplitL "client ts".
   + iExists (S n). iFrame. by eauto.
   + rewrite /rem_mapsto. case: b' => //.
-    case is_ok: cst_ok => //=.
-    iPoseProof (handshake_done_agree with "key handshake done'") as "<-".
-    iDestruct "free" as "(%γ & key' & free)".
-    iApply "up".
-    by iPoseProof (wf_key_agree with "handshake key key'") as "<-".
+    case: bool_decide_reflect => // ok.
+    iPoseProof (session_agree with "sessR handshake") as "->" => //.
+    iDestruct ("free" with "[//] [//]") as "{free} (%γ'' & sessI' & free)".
+    iPoseProof (session_agree_name with "sessI' handshake") as "(_ & ->)" => //.
+    by iApply "up".
 Qed.
 
 End Verif.
