store/client_proofs/store.v
@@ -5,7 +5,7 @@ From iris.algebra Require Import agree auth csum gset gmap excl frac.
 From iris.algebra Require Import max_prefix_list.
 From iris.heap_lang Require Import notation proofmode.
 From cryptis Require Import lib version term cryptis primitives tactics.
-From cryptis Require Import role session pk_auth pk_dh.
+From cryptis Require Import role dh_auth.
 From cryptis.store Require Import impl shared db.
 From cryptis.store.client_proofs Require Import common.
 
@@ -20,8 +20,6 @@ Notation iProp := (iProp Σ).
 
 Context `{!storeG Σ}.
 
-Local Instance STORE : PK := PK_DH (λ _ _ _ _, True)%I.
-
 Implicit Types (cs : cst).
 Implicit Types kI kR kS t : term.
 Implicit Types n : nat.
@@ -30,46 +28,15 @@ Implicit Types v : val.
 
 Variable N : namespace.
 
-Lemma wp_client_get_timestamp E cs (n : nat) :
-  {{{ cst_ts cs ↦ #n }}}
-    Client.get_timestamp (repr cs) @ E
-  {{{ RET #n; cst_ts cs ↦ #n }}}.
-Proof.
-rewrite /Client.get_timestamp.
-iIntros "%Φ Hn post".
-wp_pures. wp_load. iApply "post". iModIntro. by iFrame.
-Qed.
-
-Lemma wp_client_incr_timestamp E cs (n : nat) :
-  {{{ cst_ts cs ↦ #n }}}
-    Client.incr_timestamp (repr cs) @ E
-  {{{ RET #(); cst_ts cs ↦ #(S n) }}}.
-Proof.
-iIntros "%Ψ Hn post".
-rewrite /Client.incr_timestamp; wp_pures; wp_load; wp_store.
-iApply "post"; iFrame.
-rewrite (_ : (n + 1)%Z = (S n)%nat :> Z); last by lia.
-by iFrame.
-Qed.
-
-Lemma wp_client_get_session_key E cs :
-  {{{ True }}}
-    Client.get_session_key (repr cs) @ E
-  {{{ RET (repr (Spec.mkskey (cst_key cs))); True }}}.
-Proof.
-rewrite /Client.get_session_key.
-iIntros "%Φ ? post". wp_pures. by iApply "post".
-Qed.
-
 Lemma wp_client_send_store E c cs t1 t2 t2' :
   ↑cryptisN ⊆ E →
   channel c -∗
   store_ctx N -∗
   public t1 -∗
   public t2' -∗ (* FIXME: t1 and t2' do not have to be public already *)
-  {{{ client N cs ∗ rem_mapsto cs t1 t2 }}}
+  {{{ client cs ∗ rem_mapsto cs t1 t2 }}}
     Client.send_store N c (repr cs) t1 t2' @ E
-  {{{ RET #(); client N cs ∗ rem_mapsto cs t1 t2' }}}.
+  {{{ RET #(); client cs ∗ rem_mapsto cs t1 t2' }}}.
 Proof.
 rewrite /Client.send_store /rem_mapsto.
 iIntros "% #chan_c (_ & #? & _) #p_t1 #p_t2' !> %Φ [client mapsto] post".
@@ -88,7 +55,7 @@ iPoseProof ("post" with "[client ts mapsto]") as "post".
 iApply (wp_send with "[//] [#]") => //. iClear "post".
 iModIntro. iApply public_TEncIS => //.
 - by rewrite minted_TKey.
-- iModIntro. iExists (cst_name cs), n, t1, t2', (cst_ok cs).
+- iModIntro. iExists n, t1, t2', cs, (cst_name cs).
   do 5?iSplit => //.
 - rewrite minted_of_list /= minted_TInt; do ![iSplit => //];
   by iApply public_minted.
@@ -100,9 +67,9 @@ Lemma wp_client_ack_store E c cs :
   ↑cryptisN ⊆ E →
   channel c -∗
   store_ctx N -∗
-  {{{ client N cs }}}
+  {{{ client cs }}}
     Client.ack_store N c (repr cs) @ E
-  {{{ RET #(); client N cs }}}.
+  {{{ RET #(); client cs }}}.
 Proof.
 iIntros "% #chan_c (_ & _ & #? & _) !> %Φ client post".
 rewrite /Client.ack_store. wp_pures.
@@ -127,9 +94,9 @@ Lemma wp_client_store E c cs t1 t2 t2' :
   store_ctx N -∗
   public t1 -∗
   public t2' -∗
-  {{{ client N cs ∗ rem_mapsto cs t1 t2 }}}
+  {{{ client cs ∗ rem_mapsto cs t1 t2 }}}
     Client.store N c (repr cs) t1 t2' @ E
-  {{{ RET #(); client N cs ∗ rem_mapsto cs t1 t2' }}}.
+  {{{ RET #(); client cs ∗ rem_mapsto cs t1 t2' }}}.
 Proof.
 iIntros "% #chan_c #ctx #p_t1 #p_t2 !> %Φ [client mapsto] post".
 rewrite /Client.store.
