store/server_proofs.v
@@ -5,7 +5,7 @@ From iris.algebra Require Import agree auth csum gset gmap excl frac.
 From iris.algebra Require Import max_prefix_list.
 From iris.heap_lang Require Import notation proofmode.
 From cryptis Require Import lib version term cryptis primitives tactics.
-From cryptis Require Import role session pk_auth pk_dh.
+From cryptis Require Import role dh_auth.
 From cryptis.store Require Import impl shared alist db.
 From cryptis.store.server_proofs
   Require Import load store create.
@@ -21,8 +21,6 @@ Notation iProp := (iProp Σ).
 
 Context `{!storeGS Σ}.
 
-Local Instance STORE : PK := PK_DH (λ _ _ _ _, True)%I.
-
 Implicit Types (cs : cst) (ss : sst).
 Implicit Types kI kR kS t : term.
 Implicit Types n : nat.
@@ -35,9 +33,9 @@ Lemma wp_server_conn_handler_body E c ss :
   ↑cryptisN ⊆ E →
   channel c -∗
   store_ctx N -∗
-  {{{ server N ss }}}
+  {{{ server ss }}}
     Server.conn_handler_body N c (repr ss) @ E
-  {{{ v, RET v; server N ss }}}.
+  {{{ v, RET v; server ss }}}.
 Proof.
 iIntros "% #chan_c #ctx !> %Φ state post". rewrite /Server.conn_handler_body.
 wp_pures. wp_bind (recv _). iApply wp_recv => //.
@@ -61,7 +59,7 @@ Lemma wp_server_conn_handler E c ss :
   ↑cryptisN ⊆ E →
   channel c -∗
   store_ctx N -∗
-  {{{ server N ss }}}
+  {{{ server ss }}}
     Server.conn_handler N c (repr ss) @ E
   {{{ v, RET v; False }}}.
 Proof.
@@ -77,55 +75,39 @@ Lemma wp_server_listen E c kR dq ph T :
   ↑cryptisN ⊆ E →
   ↑N ⊆ E →
   {{{ cryptis_ctx ∗ channel c ∗ store_ctx N ∗
-      public (TKey Enc kR) ∗ ●H{dq|ph} T }}}
-    Server.listen N c (TKey Dec kR) (TKey Enc kR) @ E
+      public (TKey Dec kR) ∗ ●H{dq|ph} T }}}
+    Server.listen N c (TKey Enc kR) (TKey Dec kR) @ E
   {{{ RET #(); False }}}.
 Proof.
 iIntros "% %". iLöb as "IH".
 iIntros "%Φ (#? & #chan_c & #ctx & #p_ek & hon) post".
-wp_pures. wp_rec. wp_pures. wp_bind (pk_dh_resp _ _ _ _).
-iAssert (pk_dh_ctx N (λ _ _ _ _, True)%I) as "#?".
+wp_pures. wp_rec. wp_pures. wp_bind (responder _ _ _ _).
+iAssert (dh_auth_ctx (N.@"auth")) as "#?".
   by iDestruct "ctx" as "(_ & _ & _ & _ & _ & _ & _ & ?)".
-iApply (wp_pk_dh_resp with "[# //] [# //] [# //] [# //] [hon]") => //.
-  iFrame. by eauto.
+iApply (wp_responder inhabitant
+         with "[# //] [# //] [# //] [# //] [hon]") => //;
+  try by solve_ndisj.
 iIntros "!> %res (hon & resP)". case: res => [[pkI kS]|]; wp_pures; last first.
   iApply ("IH" with "[hon] [$]"). iFrame. by eauto.
-iDestruct "resP" as "(%kI & -> & #p_pkI & #s_kS & _ & #sessW & key)".
-wp_tag. wp_bind (mkskey _). iApply wp_mkskey. wp_pures.
-wp_bind (Fork _). iApply (wp_fork with "[key]"); last first.
+iDestruct "resP" as "(%kI & -> & #m_kI & #m_kS & #sessR & #sec_key)".
+wp_bind (Fork _). iApply wp_fork; last first.
   iModIntro. wp_pures. iApply ("IH" with "[-post] post"). iFrame.
   by eauto.
 iClear "IH". iModIntro. rewrite /Server.wait_init. wp_pures.
-iRevert "key". iApply wp_sess_recv => //.
-  by rewrite minted_tag.
-iIntros "!> %t key #p_t".
+iAssert True%I as "I"; first by []. iRevert "I". iApply wp_sess_recv => //.
+iIntros "!> %t _ #p_t".
 wp_pures. wp_bind (AList.empty _).
 iApply AList.wp_empty => //. iIntros "!> %kvs %kvs0".
 wp_alloc ldb as "Hdb". wp_pures.
 wp_alloc ts as "Hts".
-iDestruct (initE with "[//] p_t") as "{p_t} p_t".
-pose (ss := {| sst_ts := ts;
-               sst_key := Spec.tag (nroot.@"keys".@"sym") kS;
-               sst_db := ldb;
-               sst_ok := in_honest kI kR T |}).
-iAssert (handshake_done N (sst_key ss) (sst_ok ss)) as "#done".
-{ iExists kI, kR, kS, ph, T; eauto. }
-iAssert (▷ server N ss)%I with "[Hts Hdb key]" as "state".
-{ iExists 0, kvs, ∅. iFrame.
-  rewrite minted_tag /= big_sepM_empty.
-  do 4!iSplitR => //.
-  case e_ok: in_honest => //.
-  iDestruct "key" as "(#sec & _ & #key)".
-  iAssert (∀ kt, public (TKey kt (sst_key ss)) -∗ ◇ False)%I as "{sec} sec".
-  { iIntros "%kt #p_kS'".
-    iPoseProof (public_sym_keyE with "[//] p_kS'") as ">sym".
-    by iApply "sec". }
-  iDestruct "p_t" as "[p_t|p_t]".
-    by iDestruct ("sec" with "p_t") as ">[]".
-  iModIntro. iDestruct "p_t" as "(%ok & %γ & #done' & frag)".
-  iPoseProof (handshake_done_session_key with "done' key") as "->".
-  rewrite e_ok.
-  iExists γ. eauto. }
+iDestruct (initE with "[//] [//] [//] p_t") as "{p_t} p_t".
+set si := SessInfo _ _ _ _ _.
+pose (ss := {| sst_si := si;
+               sst_ts := ts;
+               sst_db := ldb; |}).
+iAssert (▷ server ss)%I with "[Hts Hdb]" as "state".
+{ iExists _, 0, kvs, ∅. iFrame.
+  rewrite big_sepM_empty. do 5!iSplitR => //. }
 wp_pures.
 iApply (wp_server_conn_handler _ ss with "[#] [#] [$]") => //.
 by iIntros "!> % []".
