store/server_proofs/create.v
@@ -5,7 +5,7 @@ From iris.algebra Require Import agree auth csum gset gmap excl frac.
 From iris.algebra Require Import max_prefix_list.
 From iris.heap_lang Require Import notation proofmode.
 From cryptis Require Import lib version term cryptis primitives tactics.
-From cryptis Require Import role session pk_auth pk_dh.
+From cryptis Require Import role dh_auth.
 From cryptis.store Require Import impl shared alist db.
 
 Set Implicit Arguments.
@@ -18,8 +18,6 @@ Context `{!cryptisGS Σ, !heapGS Σ, !sessionGS Σ}.
 Notation iProp := (iProp Σ).
 
 Context `{!storeGS Σ}.
-
-Local Instance STORE : PK := PK_DH (λ _ _ _ _, True)%I.
 
 Implicit Types (cs : cst) (ss : sst).
 Implicit Types kI kR kS t : term.
@@ -34,17 +32,17 @@ Lemma wp_server_handle_create E c ss m :
   channel c -∗
   store_ctx N -∗
   public m -∗
-  {{{ server N ss }}}
+  {{{ server ss }}}
     Server.handle_create N c (repr ss) m @ E
-  {{{ (v : option val), RET (repr v); server N ss }}}.
+  {{{ (v : option val), RET (repr v); server ss }}}.
 Proof.
 iIntros "%sub #chan_c #ctx #p_m !> %Φ state post".
 rewrite /Server.handle_create. wp_pures.
-iDestruct "state" as "(%n & %kvs & %db & #handshake & #minted_key & ts &
-                       db & %kvs_db & #pub_db & #view)".
+iDestruct "state" as "(%γ & %n & %kvs & %db & #sessR & #key_sec & #minted_key
+                       & ts & kvs & %kvs_db & #pub_db & #view)".
 wp_load. wp_pures. wp_load. wp_pures.
-iAssert (server N ss) with "[ts db view]" as "state".
-{ iExists n, kvs, db. iFrame. eauto. }
+iAssert (server ss) with "[ts kvs view]" as "state".
+{ iExists _, n, kvs, db. iFrame. eauto 8. }
 wp_tsdec m; wp_pures; last by iApply ("post" $! None).
 wp_list_of_term m; wp_pures; last by iApply ("post" $! None).
 wp_list_match => [timestamp t1 t2 ->| _]; wp_pures; last by iApply ("post" $! None).
@@ -57,57 +55,52 @@ wp_bind (AList.find _ _). iApply AList.wp_find => //.
 iIntros "!> _".
 iDestruct "ctx" as "(_ & _ & _ & _ & _ & ? & ? & _)".
 wp_bind (match: _ with InjL <> => _ | InjR <> => _ end)%E.
-iApply (wp_wand _ _ _ (λ v, server N ss ∗ ∃ b : bool,
+iApply (wp_wand _ _ _ (λ v, server ss ∗ ∃ b : bool,
   ⌜v = #(((if b then 1 else 0) : Z))⌝ ∗
   (⌜b = false⌝ ∨
    ⌜b = true⌝ ∗
-   if sst_ok ss then
-     ∃ γ, wf_key N (sst_key ss) γ ∗ DB.free_at γ n t1
-   else True))%I with "[state]").
+   □ (⌜session_ok ss⌝ -∗ ∃ γ', session ss Init γ' ∗ DB.free_at γ' n t1)))%I
+  with "[state]").
 { case db_t1: (db !! t1) => [t2'|]; wp_pures;
     first by iFrame; iExists false; eauto.
-  iDestruct "state" as "(%n' & %kvs' & %db' & _ & _ & ts & db & _ & _ & _)".
+  iDestruct "state" as "(% & %n' & %kvs' & %db' & _ & _ & _ & ts & kvs & _ & _)".
   wp_bind (AList.insert _ _ _). iApply AList.wp_insert => //.
   iIntros "!> %kvs'' %kvs''_db'". wp_store. wp_pures.
   iDestruct (public_TEncE with "p_m [//]") as "{p_m} [p_m|p_m]".
-  - case is_ok: sst_ok.
-    { iDestruct "view" as "(%γ & (#contra & _) & _)".
-      iDestruct "p_m" as "[p_k _]".
-      iDestruct ("contra" with "p_k") as ">[]". }
+  - iDestruct "p_m" as "[p_k p_m]".
+    iDestruct ("key_sec" with "p_k") as ">%".
     wp_store.
     have -> : (n + 1)%Z = S n :> Z by lia.
-    iModIntro. iSplit; last by iExists true; eauto.
-    iExists (S n), kvs'', _. iFrame. rewrite is_ok.
-    do 4!iSplit => //.
-    iApply big_sepM_insert_2 => //.
-    rewrite public_of_list /=.
-    by iDestruct "p_m" as "(_ & _ & ? & ? & _)"; eauto.
+    iModIntro. iSplitL.
+    { iExists _, (S n), kvs'', (<[t1 := t2]>db). iFrame.
+      do 5!iSplit => //.
+      + iApply big_sepM_insert_2 => //.
+        rewrite public_of_list /=.
+        by iDestruct "p_m" as "(_ & ? & ? & _)"; eauto.
+      + iIntros "%ok". tauto. }
+    iExists true. iSplit => //. iRight. iSplit => //.
+    iIntros "!> %"; tauto.
   - iDestruct "p_m" as "(#p_m & _)". wp_store.
     have -> : (n + 1)%Z = S n :> Z by lia.
-    iDestruct "p_m" as "(%γ & %n'' & %t1' & %t2' & %ok & %e & handshake' &
-                         wf & p_t1 & p_t2 & t1_t2)".
+    iDestruct "p_m" as "(%n'' & %t1' & %t2' & %si & %γ' & %e & %e_kS &
+                         sessI & p_t1 & p_t2 & t1_t2)".
     case/Spec.of_list_inj: e => e <- <- {t1' t2'}.
     have {n'' e} <- : n = n'' by lia.
-    case is_ok: sst_ok => //; last first.
-    { iSplitL; last by iExists true; eauto.
-      iModIntro. iExists (S n), kvs'', _. iFrame. rewrite is_ok.
-      do 4!iSplit => //.
-      iApply big_sepM_insert_2 => //.
-      by eauto. }
-    iDestruct "view" as "(%γ' & wf' & view)".
-    iPoseProof (handshake_done_agree with "wf' handshake handshake'")
-      as "<-".
-    iPoseProof (wf_key_agree with "handshake wf' wf") as "->".
     iSplitL.
-    + iModIntro.
-      iExists (S n), kvs'', _. iFrame. rewrite is_ok.
-      do 4!iSplit => //.
-      * iApply big_sepM_insert_2 => //.
-        by eauto.
-      * iExists γ. iSplit => //. by iApply DB.create_server.
-    + iExists true. iSplitR => //.
-      iRight. iSplitR => //. iExists γ. iModIntro. iSplit => //.
-      by iApply DB.free_atI. }
+    { iExists γ, (S n), _, _. iFrame. iModIntro. do !iSplit => //.
+      - iApply big_sepM_insert_2; eauto.
+      - iIntros "%ok".
+        iDestruct ("view" with "[//]") as "{view} (%γ'' & sessI' & view)".
+        iPoseProof (session_agree with "sessI sessR") as "->" => //.
+        iPoseProof (session_agree_name with "sessI sessI'") as "(_ & ->)" => //.
+        iExists _. iSplit => //.
+        by iApply DB.create_server. }
+    iModIntro. iExists true. iSplit => //. iRight. iSplit => //.
+    iIntros "!> %ok".
+    iDestruct ("view" with "[//]") as "{view} (%γ'' & sessI' & view)".
+    iPoseProof (session_agree with "sessI sessR") as "->" => //.
+    iPoseProof (session_agree_name with "sessI sessI'") as "(_ & ->)" => //.
+    iExists _. iSplit => //. by iApply DB.free_atI. }
 iIntros "%v (state & %b & -> & #vP)".
 wp_pures. wp_bind (tint _). iApply wp_tint. wp_list.
 wp_bind (tint _). iApply wp_tint. wp_list. wp_term_of_list.
@@ -116,7 +109,7 @@ iAssert (▷ (public t1 ∗ public t2))%I as "[p_t1 p_t2]".
     - rewrite public_of_list /=. iDestruct "p_m" as "(_ & ? & ? & _)".
       by eauto.
     - iDestruct "p_m" as "(#p_m & _)". iModIntro.
-      iDestruct "p_m" as "(%γ & %n'' & %t1' & %t2' & %ok & %e &
+      iDestruct "p_m" as "(%n'' & %t1' & %t2' & %si & %γ' & %e &
                            _ & ? & ? & ? & _)".
       by case/Spec.of_list_inj: e => _ <- <-; eauto. }
 wp_pures. wp_tsenc. wp_bind (send _ _).
@@ -126,14 +119,10 @@ iModIntro. iApply public_TEncIS => //.
 - rewrite minted_TKey.
   iPoseProof (public_minted with "p_m") as "{p_m} p_m".
   by rewrite minted_TEnc; iDestruct "p_m" as "[??]".
-- iModIntro. iExists n, t1, t2, b, (sst_ok ss). iSplit => //.
-  iSplit => //.
-  case: sst_ok => //.
-  iDestruct "view" as "(%γ & key & view)".
-  iExists γ. iSplit => //.
-  iDestruct "vP" as "[->| (-> & vP)]" => //.
-  iDestruct "vP" as "(%γ' & key' & free)".
-  by iPoseProof (wf_key_agree with "handshake key key'") as "->".
+- iModIntro. iExists n, t1, t2, b, ss, γ. do !iSplit => //.
+  iIntros "%ok %b_holds".
+  iDestruct "vP" as "[->|(_ & #vP)]" => //.
+  by iApply "vP".
 - iPoseProof (public_minted with "p_m") as "m_m".
   rewrite minted_TEnc minted_tag !minted_of_list /= !minted_TInt.
   iDestruct "m_m" as "(? & _ & ? & ? & _)". by eauto.
