store/server_proofs/load.v
@@ -5,7 +5,7 @@ From iris.algebra Require Import agree auth csum gset gmap excl frac.
 From iris.algebra Require Import max_prefix_list.
 From iris.heap_lang Require Import notation proofmode.
 From cryptis Require Import lib version term cryptis primitives tactics.
-From cryptis Require Import role session pk_auth pk_dh.
+From cryptis Require Import role dh_auth.
 From cryptis.store Require Import impl shared alist db.
 
 Set Implicit Arguments.
@@ -18,8 +18,6 @@ Context `{!cryptisGS Σ, !heapGS Σ, !sessionGS Σ}.
 Notation iProp := (iProp Σ).
 
 Context `{!storeGS Σ}.
-
-Local Instance STORE : PK := PK_DH (λ _ _ _ _, True)%I.
 
 Implicit Types (cs : cst) (ss : sst).
 Implicit Types kI kR kS t : term.
@@ -34,17 +32,17 @@ Lemma wp_server_handle_load E c ss m :
   channel c -∗
   store_ctx N -∗
   public m -∗
-  {{{ server N ss }}}
+  {{{ server ss }}}
     Server.handle_load N c (repr ss) m @ E
-  {{{ (v : option val), RET (repr v); server N ss }}}.
+  {{{ (v : option val), RET (repr v); server ss }}}.
 Proof.
 iIntros "%sub #chan_c #ctx #p_m !> %Φ state post".
 rewrite /Server.handle_load. wp_pures.
-iDestruct "state" as "(%n & %kvs & %db & #handshake & #minted_key & ts &
+iDestruct "state" as "(%γ & %n & %kvs & %db & #sessR & #key & #minted_key & ts &
                        db & %kvs_db & #pub_db & #view)".
 wp_load. wp_pures. wp_load. wp_pures.
-iAssert (server N ss) with "[ts db view]" as "state".
-{ iExists n, kvs, db. iFrame. eauto. }
+iAssert (server ss) with "[ts db view]" as "state".
+{ iExists γ, n, kvs, db. iFrame. eauto 8. }
 wp_tsdec m; wp_pures; last by iApply ("post" $! None).
 wp_list_of_term m; wp_pures; last by iApply ("post" $! None).
 wp_list_match => [timestamp t1 ->| _]; wp_pures; last by iApply ("post" $! None).
@@ -65,11 +63,11 @@ iApply public_TEncIS => //.
 - rewrite minted_TKey.
   iPoseProof (public_minted with "p_m") as "{p_m} p_m".
   by rewrite minted_TEnc; iDestruct "p_m" as "[??]".
-- iModIntro. iExists n, (sst_ok ss), t1, t2. iSplit => //.
-  do 2!iSplit => //.
-  case: sst_ok => //.
-  iDestruct "view" as "(%γ & key & view)".
-  iExists γ. iSplit => //. iApply DB.load_server; eauto.
+- iModIntro. iExists n, t1, t2, ss, γ. iSplit => //.
+  do 3!iSplit => //.
+  iIntros "%ok".
+  iDestruct ("view" with "[//]") as "{view} (%γ' & sessI & view)".
+  iExists γ'. iSplit => //. iApply DB.load_server; eauto.
 - rewrite minted_of_list /= minted_TInt -[minted t1]public_minted.
   rewrite -[minted t2]public_minted; eauto.
 - iIntros "!> _". by rewrite public_of_list /= public_TInt; eauto.
