store/server_proofs/store.v
@@ -5,7 +5,7 @@ From iris.algebra Require Import agree auth csum gset gmap excl frac.
 From iris.algebra Require Import max_prefix_list.
 From iris.heap_lang Require Import notation proofmode.
 From cryptis Require Import lib version term cryptis primitives tactics.
-From cryptis Require Import role session pk_auth pk_dh.
+From cryptis Require Import role dh_auth.
 From cryptis.store Require Import impl shared alist db.
 
 Set Implicit Arguments.
@@ -18,8 +18,6 @@ Context `{!cryptisGS Σ, !heapGS Σ, !sessionGS Σ}.
 Notation iProp := (iProp Σ).
 
 Context `{!storeGS Σ}.
-
-Local Instance STORE : PK := PK_DH (λ _ _ _ _, True)%I.
 
 Implicit Types (cs : cst) (ss : sst).
 Implicit Types kI kR kS t : term.
@@ -47,9 +45,9 @@ Lemma wp_server_handle_store E c ss m :
   channel c -∗
   store_ctx N -∗
   public m -∗
-  {{{ server N ss }}}
+  {{{ server ss }}}
     Server.handle_store N c (repr ss) m @ E
-  {{{ (v : option val), RET (repr v); server N ss }}}.
+  {{{ (v : option val), RET (repr v); server ss }}}.
 Proof.
 iIntros "%sub #chan_c #ctx #p_m !> %Φ state post".
 rewrite /Server.handle_store. wp_pures.
@@ -58,34 +56,37 @@ wp_list_of_term m; wp_pures; last by iApply ("post" $! None).
 wp_list_match => [n' t1 t2 ->|_]; wp_pures; last by iApply ("post" $! None).
 wp_bind (to_int _). iApply wp_to_int.
 case: Spec.to_intP => [ {}n' -> | _]; wp_pures; last by iApply ("post" $! None).
-iDestruct "state" as "(%n & %kvs & %db & #handshake & #minted_key & ts &
-                       db & %kvs_db & #pub_db & view)".
+iDestruct "state" as "(%γ & %n & %kvs & %db & #sessR & #sec_key &
+                       #minted_key & ts & db & %kvs_db & #pub_db & view)".
 wp_load. wp_pures.
 case: bool_decide_reflect => [[<-]|ne]; wp_pures; last first.
 { iModIntro. iApply ("post" $! None).
-  iExists n, kvs, db. iFrame. by eauto. }
+  iExists γ, n, kvs, db. iFrame. by eauto. }
 wp_load. wp_pures.
 replace (n + 1)%Z with (S n : Z) by lia.
 wp_store. wp_load. wp_bind (AList.insert _ _ _).
 wp_pures. iApply AList.wp_insert; eauto. iIntros "!> %kvs' %kvs'_db'".
-iDestruct (store_predE with "handshake [#] [//] p_m") as "(p_t1 & p_t2 & wf')".
-{ case: sst_ok => //.
-  iDestruct "view" as "(%γ & ? & ?)". eauto. }
+iDestruct (store_predE with "[//] sessR sec_key [#] p_m") as "(p_t1 & p_t2 & wf')".
+{ case: (decide (session_ok ss)) => [ok|not_ok].
+  - iDestruct ("view" with "[//]") as "(% & #? & ?)". eauto.
+  - iIntros "!> %". tauto. }
 wp_store. wp_bind (tint _). iApply wp_tint.
 wp_tsenc.
 iApply wp_fupd.
 wp_bind (send _ _). iApply wp_send => //.
 { iModIntro. iApply ack_storeI => //. }
 wp_pures. iApply ("post" $! (Some #())).
-iExists (S n), kvs', (<[t1 := t2]>db). iFrame.
+iExists γ, (S n), kvs', (<[t1 := t2]>db). iFrame.
 do 4!iSplitR => //.
+iSplitR.
 { iModIntro. iApply big_sepM_insert_2 => //. eauto. }
-case: sst_ok; eauto.
-iDestruct "wf'" as "(%γ1 & wf1 & update)".
-iDestruct "view" as "(%γ2 & #wf2 & #view)".
-iPoseProof (wf_key_agree with "handshake wf1 wf2") as "<-".
+case: (decide (session_ok ss)) => [ok|not_ok]; last first.
+{ iIntros "!> %". tauto. }
+iDestruct ("wf'" with "[//]") as "(%γ1 & sessI1 & update)".
+iDestruct ("view" with "[//]") as "(%γ2 & #sessI2 & #view)".
+iPoseProof (session_agree_name with "sessI1 sessI2") as "(_ & ->)" => //.
 iPoseProof (DB.update_server with "view update") as "view'".
-iModIntro. iExists γ1. iSplit => //.
+iIntros "!> _". iExists _. iSplit => //.
 Qed.
 
 End Verif.
